tests/lean/Tutorial/Exercises.lean
@@ -69,7 +69,7 @@ open CList
     By putting this definition in the namespace `CList`, we give the possibility of using the `.`
     notation: if `x` has type `CList α` we can write `x.toList` instead of `toList x`.
  -/
-@[simp, scalar_tac_simps, simp_lists_simps] def CList.toList {α : Type} (x : CList α) : List α :=
+@[simp, scalar_tac_simps, simp_lists_simps, grind] def CList.toList {α : Type} (x : CList α) : List α :=
   match x with
   | CNil => []
   | CCons hd tl => hd :: tl.toList
@@ -374,12 +374,6 @@ set_option pp.coercions true
 
    Small preparation for theorem `list_nth_mut1`.
  -/
-
-/- The notation `l[i]!` stands for `getElem! l`, and is the `i`th element of list `l`.
-
-   We deactivate the simp lemma below as it replaces terms of the shape `l[i]!` with more
-   complicated terms: in the present case it is more annoying than anything. -/
-attribute [-simp] List.getElem!_eq_getElem?_getD
 
 /- Reasoning about `List.index`.
 
